\documentclass{beamer} 
\usetheme{Berlin}
\usepackage{showexpl} 
\usepackage{tikz}
\usepackage{chemfig}
\usepackage[utf8]{inputenc}

\usepackage{circuitikz}
\usepackage[english]{babel}
\usepackage{blindtext}
\usepackage{multicol}
\usepackage{ragged2e}



\title{Latex}
\subtitle{Describe The Document !}



\lstloadlanguages{[LaTeX]Tex} 
\lstset{% 
     basicstyle=\ttfamily\small, 
     commentstyle=\itshape\ttfamily\small, 
     showspaces=false, 
     showstringspaces=false, 
     breaklines=true, 
     breakautoindent=true, 
     captionpos=t 
} 


\begin{document} 


\frame {
		\titlepage
	}




%%%%%%%%%%%%%%%%%%%%%%%%%%%%%%%%%%%%%%%%%%%

\frame
{
\frametitle{Seamless Graphics and Text mixture } 

\textbf{Question :} The slant height of a right circular cone is 3 cm. Find the height of cone, if its volume is the greatest.\\
%----------------------------------------
\vspace{0.4cm}
\textbf{Solution :} Let r  and x  be the base-radius and the height of the cone respectively. Then volume of the cone f(x) is given by

\begin{equation} \nonumber
\begin{alignedat}{4}
f(x) &= \frac{1}{3}\pi r^2x\\
&= \frac{\pi}{3}(3^2-x^2)x\\
&= \frac{\pi}{3}(9x - x^3)\\
\therefore f'(x) &=  \frac{\pi}{3}(9 - 3x^2)\\
\end{alignedat}
%\vrule
\quad\quad\quad
\begin{alignedat}{4}
\begin{tikzpicture}[scale=0.8]
\filldraw[fill=gray!20](0,0) ellipse (2cm and 0.6cm);
\draw (0,0) -- node[below] {\ \ \ $x$}(0,3.5);
\draw (0,0)  -- node[below] {\ \ \ $r$} (-2,0);
\draw  (-2,0) --node[above] {3\ \ }(0,3.5);
\draw  (2,0) -- (0,3.5);
\end{tikzpicture}\\\\
\end{alignedat}
\end{equation}
}

%%%%%%%%%%%%%%%%%%%%%%%%%%%%%%%%%%%%%%%%%%%%

\frame
{
\textbf{Question :} 
$\begin{aligned}[t] 
\text{If \ } x + \sqrt{xy} + y = 1 \text{\ , \  find \ \  } \frac{dy}{dx}
\end{aligned}$

\textbf{Answer:}
\begin{equation} \nonumber
\begin{alignedat}{4}
& \text{Given \ } x + \sqrt{xy} + y = 1 \\
& \text{Differentiating w.r.t. x \ }\\
& 1 + \frac{1}{2\sqrt{xy}} \left( x\frac{dy}{dx}+y \right)+\frac{dy}{dx}=0 \\
& \therefore 1 + \frac{x}{2\sqrt{xy}} \frac{dy}{dx}+ \frac{y}{2\sqrt{xy}}+\frac{dy}{dx}=0 \\
& \therefore \left(\frac{x}{2\sqrt{xy}}+1\right) \frac{dy}{dx}=-1-\frac{y}{2\sqrt{xy}}\\
\end{alignedat}
\,
\vrule
\, 
\begin{alignedat}{4}
& \therefore \left(\frac{x+2\sqrt{xy}}{2\sqrt{xy}}\right) \frac{dy}{dx}=-\frac{2\sqrt{xy}+y}{2\sqrt{xy}}\\
& \therefore  (x+2\sqrt{xy}\,)\ \frac{dy}{dx}= -2\sqrt{xy}-y \\
& \therefore \frac{dy}{dx} =-\,\frac{x+2\sqrt{xy}}{2\sqrt{xy}+y}  \\
& \\
& \\
\end{alignedat}
\end{equation}

%%%%%%%%%%%%%%%%%%%%%%%%%%%%%%%%%%%%%%%%%%%%

}



\end{document}