\documentclass[17pt]{extarticle}
\usepackage{amsmath, amssymb}
\usepackage{nccmath}
\usepackage{cancel}
\usepackage[a4paper, total={8in, 11.38in},top=2mm,left=27mm,bottom=2mm,right=5mm]{geometry}
\usepackage{tikz}
\usepackage{titlesec}

\titleformat{\section}
{\normalfont\normalsize\bfseries}{\thesection}{1em}{}
\titleformat{\subsection}
{\normalfont\normalsize\bfseries}{\thesection}{1em}{}

\begin{document}

\noindent
\begin{fleqn} 

%%%%%%%%%%%%%%%%%%%%%%%%%%%%%%%%%%%%%%%%%%%%%%%%%%%%%%%%%%%%%%%%

\section{Question} 
Form the differential equation by eliminating the arbitrary constant from the relation $ x^3 + y^3 = 4ax$

%----------------------------------------
\subsection*{Answer}
\begin{equation} \nonumber
\begin{alignedat}{4}
&  x^3 + y^3 = 4ax  \quad\quad\quad \cdots (1)  \\
& \text{Differentiating w.r.t. x \ }\\
& 3x^2 + 3y^2 \frac{dy}{dx}= 4a \\
& 3x^2 + 3y^2\frac{dy}{dx}= \frac{x^3+y^3}{x} \quad \cdots by \ (1) \quad \\
\end{alignedat}
\,
\vrule
\quad
\, 
\begin{alignedat}{4}
& 3x^3 + 3xy^2\frac{dy}{dx}=  x^2+y^3\\
& 3xy^2\frac{dy}{dx}=  y^3-2x^2\\& \\
& \\
& \\
\end{alignedat}
\end{equation}
%%%%%%%%%%%%%%%%%%%%%%%%%%%%%%%%%%%%%%%%%%%%%%%%%%%%%%%%%%%%%%%%
\section{Question} 

$\begin{aligned}[t] 
\text{If \ } x^p y^q = (x+y)^{p+q} \text{\ , \ the show that \ \  } \frac{dy}{dx}=\frac{y}{x}
\end{aligned}$

%----------------------------------------
\subsection*{Answer}
\begin{equation} \nonumber
\begin{alignedat}{4}
& \text{Given \ } x^py^q = (x+y)^{p+q} \\
& \therefore \log (x^py^q) = \log (x+y)^{p+q} \\
& \therefore p\log x + q\log y) = (p+q)\log (x+y) \\
& \text{Differentiating w.r.t. x \ }\\
& \therefore \frac{p}{x}+\frac{q}{y}\frac{dy}{dx} = \frac{p+q}{x+y}\left( 1+\frac{dy}{dx}\right)\\
& \therefore \frac{p}{x}+\frac{q}{y}\frac{dy}{dx} = \frac{p+q}{x+y} + \frac{p+q}{x+y}\,\frac{dy}{dx}\\
& \therefore \left( \frac{q}{y}-\frac{p+q}{x+y} \right)  \frac{dy}{dx} = \frac{p+q}{x+y} - \frac{p}{x}\\
\end{alignedat}
\,
\vrule
\, 
\begin{alignedat}{4}
& \therefore \frac{\cancel{qx - py}}{y} \,  \frac{dy}{dx} =  \frac{\cancel{qx - py}}{x}\\
& \therefore \frac{dy}{dx}=\frac{y}{x}\\
& \\
& \\
& \\
& \\
& \\
& \\
\end{alignedat}
\end{equation}

\begin{equation} \nonumber
\begin{alignedat}{4}
& \therefore \frac{q(x+y) - (p+q)y}{y(x+y)} \,  \frac{dy}{dx} = \frac{(p+q)x - p(x+y)}{(x+y)x}\\
& \therefore \frac{qx + qy - py - qy}{y} \,  \frac{dy}{dx} = \frac{px + qx - px - py}{x}\\
\end{alignedat}
\end{equation}


%%%%%%%%%%%%%%%%%%%%%%%%%%%%%%%%%%%%%%%%%%%%%%%%%%%%%%%%%%%%%%%%

\end{fleqn}
\end{document} 