\documentclass[17pt]{extarticle}

\usepackage{amsmath, amssymb}
\usepackage{nccmath}
\usepackage{cancel}
\usepackage[a4paper, total={8in, 11.38in},top=2mm,left=27mm,bottom=2mm,right=5mm]{geometry}
\usepackage{tikz}
\usepackage{titlesec}



\titleformat{\section}
{\normalfont\normalsize\bfseries}{\thesection}{1em}{}
\titleformat{\subsection}
{\normalfont\normalsize\bfseries}{\thesection}{1em}{}

\begin{document}

\noindent
\begin{fleqn} 

%%%%%%%%%%%%%%%%%%%%%%%%%%%%%%%%%%%%%%%%%%%%%%%%%%%%%%%%%%%%%%%%

\section{Question} 
Form the differential equation by eliminating the arbitrary constant from the relation $ x^3 + y^3 = 4ax$

%----------------------------------------
\subsection*{Answer}
\begin{equation} \nonumber
\begin{alignedat}{4}
&  x^3 + y^3 = 4ax    \hspace{3.5cm} \cdots (1)  \\
& \text{Differentiating w.r.t. x \ }\\
& 3x^2 + 3y^2 \frac{dy}{dx}= 4a \\
& 3x^2 + 3y^2\frac{dy}{dx}= \frac{x^3+y^3}{x} \quad \cdots by \ (1) \quad \\
\end{alignedat}
\,
\vrule
\quad
\, 
\begin{alignedat}{4}
& 3x^3 + 3xy^2\frac{dy}{dx}=  x^2+y^3\\
& 3xy^2\frac{dy}{dx}=  y^3-2x^2\\& \\
& \\
& \\
\end{alignedat}
\end{equation}
%%%%%%%%%%%%%%%%%%%%%%%%%%%%%%%%%%%%%%%%%%%%%%%%%%%%%%%%%%%%%%%% 

\section{Question} 
Form the differential equation by eliminating the arbitrary constant from the relation $ (y-c)^2 = cx $

%----------------------------------------
\subsection*{Answer}
\begin{equation} \nonumber
\begin{alignedat}{4}
&  (y-c)^2 = cx  \hspace{3cm} \cdots (1)  \\
& \text{Differentiating w.r.t. x \ }\\
&  2(y-c)\; \frac{dy}{dx}= c  \hspace{2.4cm} \cdots (2)\;\\
& \text{Dividing eqn (1) by eqn (2)}\\
& \frac{(y-c)^2}{2(y-c)\; \frac{dy}{dx}} =\frac{cx}{c} \\
& \therefore (y-c) = 2x\;\frac{dy}{dx} \hspace{1.5cm} \cdots (3)\\
\end{alignedat}
\,
\vrule
\quad
\, 
\begin{alignedat}{4}
& \therefore c = y - 2x\;\frac{dy}{dx} \hspace{1.7cm} \cdots (4)\\
& \text{Putting } (y-c) \text{ and }c \text{ from }\\
& (3) \text{ \& } (4)\text{ into equation (2), }\\
& 2\left( 2x\frac{dy}{dx}\right)\frac{dy}{dx}=y - 2x\;\frac{dy}{dx}\\
& \therefore 4x\left(\frac{dy}{dx}\right)^2=y - 2x\;\frac{dy}{dx}\\
& \therefore y = 2x\frac{dy}{dx}\left(1 + \frac{dy}{dx}\right)\\
\end{alignedat}
\end{equation}

%%%%%%%%%%%%%%%%%%%%%%%%%%%%%%%%%%%%%%%%%%%%%%%%%%%%%%%%%%%%%%%%

\end{fleqn}
\end{document} 